Launchbury/Sestoft.thy
@@ -2,23 +2,28 @@ theory Sestoft
 imports Terms Substitution
 begin
 
-datatype stack_elem = Arg var | Upd var
+datatype stack_elem = Arg var | Upd var | Dummy var
 
 instantiation stack_elem :: pt
 begin
-definition  "\<pi> \<bullet> x = (case x of (Arg v) \<Rightarrow> Arg (\<pi> \<bullet> v) | (Upd v) \<Rightarrow> Upd (\<pi> \<bullet> v))"
+definition  "\<pi> \<bullet> x = (case x of (Arg v) \<Rightarrow> Arg (\<pi> \<bullet> v) | (Upd v) \<Rightarrow> Upd (\<pi> \<bullet> v) | (Dummy v) \<Rightarrow> Dummy (\<pi> \<bullet> v))"
 instance
   by default (auto simp add: permute_stack_elem_def split:stack_elem.split)
 end
 
 lemma Arg_eqvt[eqvt]: "\<pi> \<bullet> (Arg v) = Arg (\<pi> \<bullet> v)"
   and Upd_eqvt[eqvt]: "\<pi> \<bullet> (Upd v) = Upd (\<pi> \<bullet> v)"
+  and Dummy_eqvt[eqvt]: "\<pi> \<bullet> (Dummy v) = Dummy (\<pi> \<bullet> v)"
   by (auto simp add: permute_stack_elem_def split:stack_elem.split)
 
 lemma supp_Arg[simp]: "supp (Arg v) = supp v"  unfolding supp_def by auto
 lemma supp_Upd[simp]: "supp (Upd v) = supp v"  unfolding supp_def by auto
+lemma supp_Dummy[simp]: "supp (Dummy v) = supp v"  unfolding supp_def by auto
 lemma fresh_Arg[simp]: "a \<sharp> Arg v = a \<sharp> v" unfolding fresh_def by auto
 lemma fresh_Upd[simp]: "a \<sharp> Upd v = a \<sharp> v" unfolding fresh_def by auto
+lemma fresh_Dummy[simp]: "a \<sharp> Dummy v = a \<sharp> v" unfolding fresh_def by auto
+lemma fv_Arg[simp]: "fv (Arg v) = fv v"  unfolding fv_def by auto
+lemma fv_Upd[simp]: "fv (Upd v) = fv v"  unfolding fv_def by auto
 
 instance stack_elem :: fs  by (default, case_tac x) (auto simp add: finite_supp)
 
@@ -44,9 +49,13 @@ inductive step :: "conf \<Rightarrow> conf \<Rightarrow> bool" (infix "\<Rightar
   app\<^sub>1:  "(\<Gamma>, App e x, S) \<Rightarrow> (\<Gamma>, e , Arg x # S)"
 | app\<^sub>2:  "(\<Gamma>, Lam [y]. e, Arg x # S) \<Rightarrow> (\<Gamma>, e[y ::= x] , S)"
 | var\<^sub>1:  "map_of \<Gamma> x = Some e \<Longrightarrow> (\<Gamma>, Var x, S) \<Rightarrow> (delete x \<Gamma>, e , Upd x # S)"
-| var\<^sub>2:  "isLam e \<Longrightarrow> (\<Gamma>, e, Upd x # S) \<Rightarrow> ((x,e)# \<Gamma>, e , S)"
-| let\<^sub>1:  "atom ` domA \<Delta> \<sharp>* (\<Gamma>, S) \<Longrightarrow> (\<Gamma>, Let \<Delta> e, S) \<Rightarrow> (\<Delta>@\<Gamma>, e , S)"
+| var\<^sub>2:  "x \<notin> domA \<Gamma> \<Longrightarrow> isLam e \<Longrightarrow> (\<Gamma>, e, Upd x # S) \<Rightarrow> ((x,e)# \<Gamma>, e , S)"
+| let\<^sub>1:  "atom ` domA \<Delta> \<sharp>* \<Gamma> \<Longrightarrow> atom ` domA \<Delta> \<sharp>* S \<Longrightarrow> (\<Gamma>, Let \<Delta> e, S) \<Rightarrow> (\<Delta>@\<Gamma>, e , S)"
 
 abbreviation steps (infix "\<Rightarrow>\<^sup>*" 50) where "steps \<equiv> step\<^sup>*\<^sup>*"
+
+lemma SmartLet_stepI:
+   "atom ` domA \<Delta> \<sharp>* \<Gamma> \<Longrightarrow> atom ` domA \<Delta> \<sharp>* S \<Longrightarrow> (\<Gamma>, SmartLet \<Delta> e, S) \<Rightarrow>\<^sup>*  (\<Delta>@\<Gamma>, e , S)"
+unfolding SmartLet_def by (auto intro: let\<^sub>1)
 
 end
